#+TITLE: SST Notes



* Study / Review
** Chapter 1
** Chapter 2
** Chapter 3
** Chapter 4
** Chapter 5
Frequency and Magnitude Response - conversions from $H[z]$ to $H[e^{j\omega}]$

* Previous

* Everlasting Exponential
$y(t) = h(t)*e^{st} = \int_{-\infty}^{\infty}{h{\tau}e^{s(t-\tau)}d\tau$
$=e^{st}\int_{-\infty}^{\infty}{h(\tau)e^{-s\tau}d\tau$ - This is the Transfer Function - $H(s)$

As a result:
$y(t) = H(s)e^{st} = H(s)[Cos(bt)+jSin(bt)]e^{at}$

Let $a=0$ and $b=w$
$s=jw$ -> $y(t)=H(jw)Cos(wt)+jH(jw)Sin(wt) = y_{real}(t) + y_{imag}(t)$

| Input (x(t))   | Output (y(t))                         |
|----------------+---------------------------------------|
| Cos(wt)        | Re{H(jw)e^{jwt}}                      |
| Cos(wt)        | \Abs{H(jw)}Cos(wt+\angle{H(jw)}       |
| Cos(wt+\theta) | \Abs{H(jw)Cos(wt+\theta+\angle{H(jw)} |

** Example
- $$H(s) = \frac{s+2}{s^{2}+5s+4}$$
- $$x(t) = 5Cos(2t+30\degree)$$
  Find the response, $y(t)$
  $$H(j2) = \frac{j2+2}{(j2)^{2}+5(j2)+4 = 0.28\angle -45\degree$$
  $$y(t) = 5(0.28)Cos(2t+30\degree - 45\degree) = 1.4Cos(2t-15\degree)$$

* Frequency Response
$H(jw) = |H(jw)|e^{j\angle{H(jw)}}$
Absolute Value - Magnitude Response
Exponential - Phase Response

** Example
- $H(s) = \frac{s+0.1}{s+5}$

- Find magnitude and phase response
- Find response to $x(t) = Cos(2t)$

  a)
  $H(jw) = \frac{jw+0.1}{jw+5}$
  $|H(jw)| = \frac{\sqrt{(jw)^{2}+(0.1)^{2}}}{\sqrt{(jw)^{2}+5^{2}}} = \frac{\sqrt{w^{2}+0.01}}{\sqrt{w^{2}+25}}$ - Magnitude
  $\angle{H(jw)} = \frac{Tan^{-1}(\frac{w}{0.1})}{Tan^{-1}(\frac{w}{5})} = Tan^{-1}(\frac{w}{5})$ - Phase Response

  b)
  Just plug in 2 for w. Its calculator work.

* Vector Plots

$H(s) = \frac{P(s)}{Q(s)} = b_{0}\frac{(s-z_{1})(s-z_{2})...(s-z_{n})}{(s-\lambda_{1})(s-\lambda_{2})...(s-\lambda_{n})}$

* Steady State Response
Remember: $H(s) = \frac{P(s)}{Q(s)} = \frac{(s-z_{1})(s-z_{2})...(s-z_{n})}{(s-\lambda_{1})(s-\lambda_{2})...(s-\lambda_{n})}$
$X(s) = \frac{1}{s-j\omega}$

$Y(s) = H(s)X(s) = \frac{P(s)}{(s-\lambda_{1})(s-\lambda_{2})...(s-\lambda_{n})}$
Partial Fraction Decomp: $Y(s) = \frac{P(j\omega)}{(j\omega-\lambda_{1})(j\omega-\lambda_{2})...(j\omega-\lambda_{n})}=\frac{P(j\omega)}{Q(j\omega)}=H(j\omega)$

$y_{ss}(t) = H(j\omega)e^{j\omega t}u(t)$
$y_{ss}(t)=Re[H(j\omega)e^{j\omega t}u(t)] = |H(j\omega)|Cos(\omega t+\angle{H(j\omega)})u(t)$

** Example
Let $H(s)=\frac{s+2}{s^{2}+5s+4}\,\,;\,\,x(t)=2+5Cos(2t+30\degree)$
Find the Steady State Response






$x_{1}(t)=2\,\,;\,\,w_{1}=0$
$H(jo)=\frac{1}{2}\angle{0\degree}$
--> $y{1}(t)=2(\frac{1}{2})$

$x_{2}(t) = 5Cos(2t+30\degree)\,\,;\,\,w_{1}=2$
$H(j2)=0.28\angle{-45\degree}$
--> $y_{2}(t)=5(0.28)Cos(2t+30\degree-45\degree)$

* Bilateral Laplace
$x_{1}(t) = e^{-at}u(t)$
$x_{2}(t) = -e^{-at}u(-t)$
$\mathbb{L}[x_{1}(t)] = \frac{1}{s+a}\,\,Re[s]>a$
$\mathbb{L}[x_{2}(t)]=\frac{1}{s+a}\,\,Re[s]<-a$
$x_1$-> Causal, RIght Sided, Pole lies on left side of ROC
$x_2$ -> Non Causal, Left sided, Pole lies on right side of ROC

Steps:
- Split $x(t)$ into Causal and Anti-Causal Regions
- Take Unilateral Transforms of $x_{c}(t)$ - causal and $x_{a}(t)$ - anti-causal
- $X_{a}(s)\rightarrow X_{a}(-s)$

** Example
$X(s) = \frac{-3}{(s+2)(s-1)} = \frac{A}{s+2} +\frac{B}{s-1} = \frac{1}{s+2} -\frac{1}{s-1}$
A. Find $x(t)$ given $-2<Re(s)<1$
B. Find $x(t)$ given $Re(s)>1$

A.
$X(s) = X_{c}(t)+X_{a}(t)$
$Ae^{-2t}u(t)+e^{t}u(t) = e^{-2t}+e^{t}u(t)$

[[file:c:/Users/Christian/Documents/GitHub/OrgFiles/Class Notes/Gimp/SST2 17MAR23.png]]

[[file:c:/Users/Christian/Documents/GitHub/OrgFiles/Class Notes/Gimp/SST 17MAR23.png]]

B.
$e^{-2t}u(t)-e^{t}u(t)$
